wip concrete state

io/MIO.Sig.fst
@@ -6,9 +6,9 @@ include CommonUtils
 include Free
 include Hist
 
-type cmds = | Openfile | Read | Close | Write | GetTrace
+type cmds = | Openfile | Read | Close | Write | GetTrace | GetST
 
-(** the io free monad does not contain the GetTrace step **)
+(** the io free monad does not contain the GetTrace/GetST steps **)
 let _io_cmds x : bool = x = Openfile || x = Read || x = Close || x = Write
 type io_cmds : Type = x:cmds{_io_cmds x}
 
@@ -44,45 +44,54 @@ type event =
 
 type trace = list event
 
-type m_cmds = x:cmds{x = GetTrace}
+type m_cmds = x:cmds{x = GetTrace || x = GetST}
 
-(** We only need GetTrace because we assume that our actions are
+(** We only need GetTrace/GetST because we assume that our actions are
 updating the trace for us. Therefore, at extraction, our actions
 should be linked with wrapped primitives that initialize a
 trace on the heap (?) and updates it with events.
 GetTrace will be linked with a function that returns the reference
 to the trace from the heap. **)
 
+(* Monitoring state. *)
+noeq
+type mst = {
+  cst : Type0;
+  models : cst -> trace -> Type0;
+}
+
 (** Is our assumption limiting how the IO effect can be used?
  What if somebody wants to use only the IO effect? Then,
 at extraction, they have to be careful to link it directly with the
 primitives, and not with the wrapped version, otherwise, they will
 suffer a performance penalty. **)
-let m_args (cmd:m_cmds) =
+let m_args (mst:mst) (cmd:m_cmds) =
   match cmd with
   | GetTrace -> unit
+  | GetST -> unit
 
-let m_res (cmd:m_cmds) (arg:m_args cmd) =
+let m_res (mst:mst) (cmd:m_cmds) (arg:m_args mst cmd) =
   match cmd with
-  | GetTrace -> trace 
+  | GetTrace -> Ghost.erased trace 
+  | GetST -> mst.cst
 
-let m_sig : op_sig m_cmds = {
-  args = m_args;
-  res = m_res;
+let m_sig (mst:mst): op_sig m_cmds = {
+  args = m_args mst;
+  res = m_res mst;
 }
 
-let _mio_cmds (cmd:cmds) : bool = _io_cmds cmd || cmd = GetTrace
+let _mio_cmds (cmd:cmds) : bool = _io_cmds cmd || cmd = GetTrace || cmd = GetST
 type mio_cmds = cmd:cmds{_mio_cmds cmd}
-let mio_sig : op_sig mio_cmds = add_sig cmds io_sig m_sig
+let mio_sig (mst:mst) : op_sig mio_cmds = add_sig cmds io_sig (m_sig mst)
 
 // THE IIO FREE MONAD
-type mio (a:Type) = free cmds mio_sig a
+type mio (mst:mst) (a:Type) = free cmds (mio_sig mst) a
 
-let mio_return (x:'a) : mio 'a =
-  free_return cmds mio_sig 'a x
+let mio_return #st (x:'a) : mio st 'a =
+  free_return cmds (mio_sig st) 'a x
 
-let mio_bind (#a:Type) (#b:Type) l k : mio b =
-  free_bind cmds mio_sig a b l k
+let mio_bind #st (#a:Type) (#b:Type) l k : mio st b =
+  free_bind cmds (mio_sig st) a b l k
 
 let convert_call_to_event
   (caller:bool)
@@ -128,7 +137,11 @@ unfold let io_pre (cmd:io_cmds) (arg:io_args cmd) (h:trace) : Type0 =
   | Write -> let (fd, _):(file_descr*string) = arg in is_open fd h
   | Close -> is_open arg h**)
 
-unfold let mio_wps (caller:bool) (cmd:mio_cmds) (arg:mio_sig.args cmd) : hist (mio_sig.res cmd arg) = fun p h ->
+unfold let mio_wps #mst (caller:bool) (cmd:mio_cmds) (arg:(mio_sig mst).args cmd) : hist ((mio_sig mst).res cmd arg) =
+  fun (p : hist_post ((mio_sig mst).res cmd arg)) h ->
   match cmd with
-  | GetTrace -> p [] h
-  | _ -> io_pre cmd arg h /\ (forall (r:mio_sig.res cmd arg). p [convert_call_to_event caller cmd arg r] r)
+  | GetTrace ->
+    let p : hist_post (Ghost.erased trace) = p in // need some handholding
+    p [] (Ghost.hide h)
+  | GetST -> forall (x:mst.cst). mst.models x h ==> p [] x // any concrete state modelling the trace
+  | _ -> io_pre cmd arg h /\ (forall (r:(mio_sig mst).res cmd arg). p [convert_call_to_event caller cmd arg r] r)
