io/MIO.Sig.Call.fst
@@ -6,5 +6,5 @@ assume val print_string2 : string -> Tot bool
 
 (** This file is replaced during linking with a file that contains the real
 implementation of the commands. **)
-let mio_call (caller:bool) (cmd:cmds) (arg:mio_sig.args cmd) : mio (mio_sig.res cmd arg) =
+let mio_call (#mst:mst) (caller:bool) (cmd:cmds) (arg:(mio_sig mst).args cmd) : mio mst ((mio_sig mst).res cmd arg) =
   Call caller cmd arg Return
